move cancel_in_hyp to HeapletwiseHyps and use actual map.eqb
instead of Axiom map__eqb

bedrock2/src/bedrock2/HeapletwiseAutoSplitMerge.v
@@ -468,121 +468,6 @@ Ltac split_range_from_hyp_default :=
 
 Ltac split_range_from_hyp_hook := split_range_from_hyp_default.
 
-Section CancelingInHyp.
-  Context {key value: Type} {mem: map.map key value} {mem_ok: map.ok mem}
-          {key_eqb: key -> key -> bool} {key_eqb_spec: Decidable.EqDecider key_eqb}.
-
-  Definition canceling_in_hyp(mAll: mem)(omAvailable: mmap mem)
-    (Ps: list (mem -> Prop))(Q: mem -> Prop) :=
-    exists mUsed, mmap.du omAvailable (mmap.Def mUsed) = mmap.Def mAll /\
-                  forall mp mq, mmap.du (mmap.Def mp) (mmap.Def mUsed) = mmap.Def mq ->
-                                seps Ps mp -> Q mq.
-
-  Lemma start_canceling_in_hyp: forall Ps (Q: mem -> Prop) omAll mAll,
-      omAll = mmap.Def mAll ->
-      (forall m, SeparationLogic.Tree.to_sep Ps m -> Q m) ->
-      canceling_in_hyp mAll omAll (SeparationLogic.Tree.flatten Ps) Q.
-  Proof.
-    unfold canceling_in_hyp. intros. exists map.empty. split.
-    - rewrite mmap.du_empty_r. exact H.
-    - intros. rewrite mmap.du_empty_r in H1. inversion H1. subst mp. clear H1.
-      eapply H0. eapply SeparationLogic.Tree.flatten_iff1_to_sep. assumption.
-  Qed.
-
-  Lemma canceling_step_in_hyp: forall (P: mem -> Prop) Ps Q mAll m path hs1 hs2,
-      with_mem m P ->
-      mem_tree_lookup hs1 path = Some m ->
-      mem_tree_remove hs1 path = Some hs2 ->
-      canceling_in_hyp mAll (interp_mem_tree hs1) (cons P Ps) Q ->
-      canceling_in_hyp mAll (interp_mem_tree hs2) Ps Q.
-  Proof.
-    unfold canceling_in_hyp. intros. fwd.
-    unfold mmap.du, mmap.of_option in H2p0. fwd.
-    epose proof (split_mem_tree H0 H1 E) as A.
-    exists (map.putmany m mUsed).
-    unfold map.du in E0. fwd.
-    unfold mmap.du, mmap.of_option in A. fwd.
-    eapply map.disjointb_spec in E1.
-    assert (map.disjoint m mUsed) as D. {
-      unfold map.du in E2. fwd. eapply map.disjointb_spec in E3.
-      unfold map.disjoint in *. intros. eapply E1. 2: eassumption.
-      rewrite map.get_putmany_dec. rewrite H2. reflexivity.
-    }
-    split.
-    - unfold map.du in E2. fwd.
-      unfold mmap.du, mmap.of_option, map.du.
-      eapply map.disjoint_putmany_l in E1. fwd.
-      replace (map.disjointb m1 (map.putmany m mUsed)) with true.
-      1: rewrite map.putmany_assoc; reflexivity.
-      symmetry. eapply map.disjointb_spec. eapply map.disjoint_putmany_r.
-      eapply map.disjointb_spec in E3. auto.
-    - intros.
-      unfold mmap.du, mmap.of_option, map.du in H2. fwd.
-      eapply map.disjointb_spec in E4. eapply map.disjoint_putmany_r in E4. fwd.
-      eapply H2p1.
-      2: {
-        eapply SeparationLogic.seps_cons. eapply sep_from_disjointb. 2,3: eassumption.
-        eapply map.disjointb_spec. apply map.disjoint_comm. assumption.
-      }
-      unfold mmap.du, mmap.of_option, map.du.
-      replace (map.disjointb (map.putmany m mp) mUsed) with true.
-      + rewrite map.putmany_assoc. f_equal. f_equal. eapply map.putmany_comm.
-        eapply map.disjoint_comm. assumption.
-      + symmetry. eapply map.disjointb_spec. eapply map.disjoint_putmany_l. auto.
-  Qed.
-
-  Lemma canceling_done_in_hyp: forall Q mAll omAvailable,
-      canceling_in_hyp mAll omAvailable nil Q ->
-      exists m, mmap.du omAvailable (mmap.Def m) = mAll /\ with_mem m Q.
-  Proof.
-    unfold canceling_in_hyp. intros. fwd. exists mUsed. split. 1: assumption.
-    eapply Hp1. 1: eapply mmap.du_empty_l. unfold seps, emp. auto.
-  Qed.
-End CancelingInHyp.
-
-Ltac start_canceling_in_hyp H :=
-  unfold merge_step in H;
-  repeat lazymatch type of H with
-    | forall m, ?A m -> ?B m => fail (* done *)
-    | forall (_: ?A), _ => let x := lazymatch open_constr:(_: A) with ?x => x end in
-                           specialize (H x)
-    end;
-  lazymatch type of H with
-  | forall m, ?A m -> ?B m =>
-      let clausetree := SeparationLogic.reify A in
-      change (forall m, SeparationLogic.Tree.to_sep clausetree m -> B m) in H;
-      lazymatch goal with
-      | D: _ = mmap.Def _ |- _ =>
-          eapply (start_canceling_in_hyp clausetree _ _ _ D) in H;
-          clear D;
-          cbn [SeparationLogic.Tree.flatten
-               SeparationLogic.Tree.interp
-               bedrock2.Map.SeparationLogic.app] in H
-      end
-  end.
-
-Ltac canceling_step_in_hyp C :=
-  lazymatch type of C with
-  | canceling_in_hyp ?mAll ?om (cons ?P ?Ps) ?Q =>
-      let H := match goal with
-               | H: with_mem _ ?P' |- _ =>
-                   let __ := match constr:(Set) with _ => syntactic_unify P P' end in H
-               end in
-      let m := lazymatch type of H with with_mem ?m _ => m end in
-      let hs := reify_mem_tree om in
-      let p := path_in_mem_tree hs m in
-      eapply (canceling_step_in_hyp P Ps Q mAll m p hs _ H) in C;
-      [ | reflexivity | reflexivity];
-      cbn [interp_mem_tree] in C;
-      clear H m
-  end.
-
-Ltac cancel_in_hyp H :=
-  start_canceling_in_hyp H;
-  repeat canceling_step_in_hyp H;
-  eapply canceling_done_in_hyp in H;
-  destruct H as (?m & ?D & ?H).
-
 Ltac merge_step_in_hyp H :=
   lazymatch type of H with
   (* Special case for records: Need to solve sideconditions SC1 and SC2 (using eq_refl).
@@ -599,6 +484,7 @@ Ltac merge_step_in_hyp H :=
       end
   | _ => idtac
   end;
+  unfold merge_step in H;
   cancel_in_hyp H.
 
 Lemma f_equal_fun[A B: Type]: forall (f g: A -> B) (x: A), f = g -> f x = g x.
