bedrock2/src/bedrock2/HeapletwiseHyps.v
@@ -24,7 +24,8 @@ Notation "m |= P" := (with_mem m P) (at level 72) : heapletwise_scope.
 
 Section HeapletwiseHyps.
   Context {key value: Type} {mem: map.map key value} {mem_ok: map.ok mem}
-          {key_eqb: key -> key -> bool} {key_eqb_spec: EqDecider key_eqb}.
+          {key_eqb: key -> key -> bool} {key_eqb_spec: EqDecider key_eqb}
+          {value_eqb: value -> value -> bool} {value_eq_dec: EqDecider value_eqb}.
 
   Lemma split_du: forall (m m1 m2: mem),
       map.split m m1 m2 <-> mmap.du m1 m2 = m.
@@ -90,7 +91,7 @@ Section HeapletwiseHyps.
 
   Lemma sep_to_with_mem_and_with_mem: forall (P Q: mem -> Prop) m,
       sep P Q m ->
-      exists m1 m2, with_mem m1 P /\ with_mem m2 Q /\ m1 \*/ m2 = m.
+      exists m1 m2, with_mem m1 P /\ with_mem m2 Q /\ mmap.du m1 m2 = m.
   Proof.
     unfold with_mem, sep, map.split. intros. fwd. do 2 eexists. ssplit.
     1,2: eassumption.
@@ -100,25 +101,25 @@ Section HeapletwiseHyps.
 
   Lemma sep_to_with_mem_and_unpacked: forall (P Q: mem -> Prop) m,
       sep P Q m ->
-      exists m1 m2, with_mem m1 P /\ Q m2 /\ m1 \*/ m2 = m.
+      exists m1 m2, with_mem m1 P /\ Q m2 /\ mmap.du m1 m2 = m.
   Proof. exact sep_to_with_mem_and_with_mem. Qed.
 
   Lemma sep_to_unpacked_and_with_mem: forall (P Q: mem -> Prop) m,
       sep P Q m ->
-      exists m1 m2, P m1 /\ with_mem m2 Q /\ m1 \*/ m2 = m.
+      exists m1 m2, P m1 /\ with_mem m2 Q /\ mmap.du m1 m2 = m.
   Proof. exact sep_to_with_mem_and_with_mem. Qed.
 
   Lemma sep_to_unpacked_and_unpacked: forall (P Q: mem -> Prop) m,
       sep P Q m ->
-      exists m1 m2, P m1 /\ Q m2 /\ m1 \*/ m2 = m.
+      exists m1 m2, P m1 /\ Q m2 /\ mmap.du m1 m2 = m.
   Proof. exact sep_to_with_mem_and_with_mem. Qed.
 
   Lemma merge_two_split_equations: forall {m} {om1 om2: mmap mem},
       om1 = mmap.Def m ->
       om2 = mmap.Def m ->
-      om1 \=/ om2 = mmap.Def m.
+      mmap.equal_union value_eqb om1 om2 = mmap.Def m.
   Proof.
-    unfold mmap.equal_union. intros. subst. destr (mmap.map__eqb m m); congruence.
+    unfold mmap.equal_union. intros. subst. destr (map.eqb value_eqb m m); congruence.
   Qed.
 
   Inductive mem_tree :=
@@ -128,7 +129,7 @@ Section HeapletwiseHyps.
   | NEqualUnion(t1 t2: mem_tree).
 
   Lemma invert_Some_eq_equal_union: forall m (om1 om2: mmap mem),
-      mmap.equal_union om1 om2 = mmap.Def m ->
+      mmap.equal_union value_eqb om1 om2 = mmap.Def m ->
       om1 = mmap.Def m /\ om2 = mmap.Def m.
   Proof.
     unfold mmap.equal_union. intros. fwd. auto.
@@ -139,7 +140,8 @@ Section HeapletwiseHyps.
     | NEmpty => mmap.Def map.empty
     | NLeaf m => mmap.Def m
     | NDisjointUnion t1 t2 => mmap.du (interp_mem_tree t1) (interp_mem_tree t2)
-    | NEqualUnion t1 t2 => mmap.equal_union (interp_mem_tree t1) (interp_mem_tree t2)
+    | NEqualUnion t1 t2 =>
+        mmap.equal_union value_eqb (interp_mem_tree t1) (interp_mem_tree t2)
     end.
 
   Fixpoint mem_tree_lookup(t: mem_tree)(path: list bool): option mem :=
@@ -451,6 +453,73 @@ Section HeapletwiseHyps.
     + eapply map.disjoint_putmany_l. rewrite map.putmany_comm.
       1: eassumption. apply map.disjoint_comm. eapply map.disjointb_spec. assumption.
   Qed.
+
+  Definition canceling_in_hyp(mAll: mem)(omAvailable: mmap mem)
+    (Ps: list (mem -> Prop))(Q: mem -> Prop) :=
+    exists mUsed, mmap.du omAvailable (mmap.Def mUsed) = mmap.Def mAll /\
+                  forall mp mq, mmap.du (mmap.Def mp) (mmap.Def mUsed) = mmap.Def mq ->
+                                seps Ps mp -> Q mq.
+
+  Lemma start_canceling_in_hyp: forall Ps (Q: mem -> Prop) omAll mAll,
+      omAll = mmap.Def mAll ->
+      (forall m, SeparationLogic.Tree.to_sep Ps m -> Q m) ->
+      canceling_in_hyp mAll omAll (SeparationLogic.Tree.flatten Ps) Q.
+  Proof.
+    unfold canceling_in_hyp. intros. exists map.empty. split.
+    - rewrite mmap.du_empty_r. exact H.
+    - intros. rewrite mmap.du_empty_r in H1. inversion H1. subst mp. clear H1.
+      eapply H0. eapply SeparationLogic.Tree.flatten_iff1_to_sep. assumption.
+  Qed.
+
+  Lemma canceling_step_in_hyp: forall (P: mem -> Prop) Ps Q mAll m path hs1 hs2,
+      with_mem m P ->
+      mem_tree_lookup hs1 path = Some m ->
+      mem_tree_remove hs1 path = Some hs2 ->
+      canceling_in_hyp mAll (interp_mem_tree hs1) (cons P Ps) Q ->
+      canceling_in_hyp mAll (interp_mem_tree hs2) Ps Q.
+  Proof.
+    unfold canceling_in_hyp. intros. fwd.
+    unfold mmap.du, mmap.of_option in H2p0. fwd.
+    epose proof (split_mem_tree H0 H1 E) as A.
+    exists (map.putmany m mUsed).
+    unfold map.du in E0. fwd.
+    unfold mmap.du, mmap.of_option in A. fwd.
+    eapply map.disjointb_spec in E1.
+    assert (map.disjoint m mUsed) as D. {
+      unfold map.du in E2. fwd. eapply map.disjointb_spec in E3.
+      unfold map.disjoint in *. intros. eapply E1. 2: eassumption.
+      rewrite map.get_putmany_dec. rewrite H2. reflexivity.
+    }
+    split.
+    - unfold map.du in E2. fwd.
+      unfold mmap.du, mmap.of_option, map.du.
+      eapply map.disjoint_putmany_l in E1. fwd.
+      replace (map.disjointb m1 (map.putmany m mUsed)) with true.
+      1: rewrite map.putmany_assoc; reflexivity.
+      symmetry. eapply map.disjointb_spec. eapply map.disjoint_putmany_r.
+      eapply map.disjointb_spec in E3. auto.
+    - intros.
+      unfold mmap.du, mmap.of_option, map.du in H2. fwd.
+      eapply map.disjointb_spec in E4. eapply map.disjoint_putmany_r in E4. fwd.
+      eapply H2p1.
+      2: {
+        eapply SeparationLogic.seps_cons. eapply sep_from_disjointb. 2,3: eassumption.
+        eapply map.disjointb_spec. apply map.disjoint_comm. assumption.
+      }
+      unfold mmap.du, mmap.of_option, map.du.
+      replace (map.disjointb (map.putmany m mp) mUsed) with true.
+      + rewrite map.putmany_assoc. f_equal. f_equal. eapply map.putmany_comm.
+        eapply map.disjoint_comm. assumption.
+      + symmetry. eapply map.disjointb_spec. eapply map.disjoint_putmany_l. auto.
+  Qed.
+
+  Lemma canceling_done_in_hyp: forall Q mAll omAvailable,
+      canceling_in_hyp mAll omAvailable nil Q ->
+      exists m, mmap.du omAvailable (mmap.Def m) = mAll /\ with_mem m Q.
+  Proof.
+    unfold canceling_in_hyp. intros. fwd. exists mUsed. split. 1: assumption.
+    eapply Hp1. 1: eapply mmap.du_empty_l. unfold seps, emp. auto.
+  Qed.
 End HeapletwiseHyps.
 
 Ltac reify_mem_tree e :=
@@ -459,7 +528,7 @@ Ltac reify_mem_tree e :=
       let t1 := reify_mem_tree e1 in
       let t2 := reify_mem_tree e2 in
       constr:(NDisjointUnion t1 t2)
-  | mmap.equal_union ?e1 ?e2 =>
+  | mmap.equal_union _ ?e1 ?e2 =>
       let t1 := reify_mem_tree e1 in
       let t2 := reify_mem_tree e2 in
       constr:(NEqualUnion t1 t2)
@@ -723,11 +792,11 @@ Ltac merge_du_step :=
   | E1: ?om1 = @mmap.Def _ _ ?Mem ?m, E2: ?om2 = mmap.Def ?m' |- _ =>
       lazymatch om1 with
       | mmap.du _ _ => idtac
-      | mmap.equal_union _ _ => idtac
+      | mmap.equal_union _ _ _ => idtac
       end;
       lazymatch om2 with
       | mmap.du _ _ => idtac
-      | mmap.equal_union _ _ => idtac
+      | mmap.equal_union _ _ _ => idtac
       end;
       lazymatch om2 with
       | context C[mmap.Def m] =>
@@ -876,9 +945,52 @@ Ltac collect_heaplets_into_one_sepclause :=
       eapply done_collecting_heaplets in D
   end.
 
+Ltac start_canceling_in_hyp H :=
+  repeat lazymatch type of H with
+    | forall m, ?A m -> ?B m => fail (* done *)
+    | forall (_: ?A), _ => let x := lazymatch open_constr:(_: A) with ?x => x end in
+                           specialize (H x)
+    end;
+  lazymatch type of H with
+  | forall m, ?A m -> ?B m =>
+      let clausetree := SeparationLogic.reify A in
+      change (forall m, SeparationLogic.Tree.to_sep clausetree m -> B m) in H;
+      lazymatch goal with
+      | D: _ = mmap.Def _ |- _ =>
+          eapply (start_canceling_in_hyp clausetree _ _ _ D) in H;
+          clear D;
+          cbn [SeparationLogic.Tree.flatten
+               SeparationLogic.Tree.interp
+               bedrock2.Map.SeparationLogic.app] in H
+      end
+  end.
+
+Ltac canceling_step_in_hyp C :=
+  lazymatch type of C with
+  | canceling_in_hyp ?mAll ?om (cons ?P ?Ps) ?Q =>
+      let H := match goal with
+               | H: with_mem _ ?P' |- _ =>
+                   let __ := match constr:(Set) with _ => syntactic_unify P P' end in H
+               end in
+      let m := lazymatch type of H with with_mem ?m _ => m end in
+      let hs := reify_mem_tree om in
+      let p := path_in_mem_tree hs m in
+      eapply (canceling_step_in_hyp P Ps Q mAll m p hs _ H) in C;
+      [ | reflexivity | reflexivity];
+      cbn [interp_mem_tree] in C;
+      clear H m
+  end.
+
+Ltac cancel_in_hyp H :=
+  start_canceling_in_hyp H;
+  repeat canceling_step_in_hyp H;
+  eapply canceling_done_in_hyp in H;
+  destruct H as (?m & ?D & ?H).
+
 Section HeapletwiseHypsTests.
   Context {key value: Type} {mem: map.map key value} {mem_ok: map.ok mem}
-          {key_eqb: key -> key -> bool} {key_eqb_spec: EqDecider key_eqb}.
+          {key_eqb: key -> key -> bool} {key_eqb_spec: EqDecider key_eqb}
+          {value_eqb: value -> value -> bool} {value_eq_dec: EqDecider value_eqb}.
 
   Hypothesis scalar: nat -> nat -> mem -> Prop.
 
@@ -938,7 +1050,7 @@ Section HeapletwiseHypsTests.
     step. step. step. step. step. step. step.
     (* split seps into separate hyps: *)
     step. step. step. step.
-    (* just for desting, join them back together: *)
+    (* just for testing, join them back together: *)
     collect_heaplets_into_one_sepclause. cbn [seps] in D.
     (* and split again: *)
     step. step. step. step.
